ContextTyping/theories/SoundnessLamBase.v
@@ -87,10 +87,10 @@ Proof.
       unfold relevant_env, lty_env_restrict_lvars.
       rewrite storeA_restrict_lookup.
       destruct (decide
-        (LVFree a ∈ relevant_lvars (CTArrow τx τ) (tret vf)))
+        (LVFree a ∈ context_tm_support (CTArrow τx τ) (tret vf)))
         as [_|Hbad]; [reflexivity|].
       exfalso. apply Hbad.
-      unfold relevant_lvars in Hu |- *.
+      unfold relevant_lvars, context_tm_support in Hu |- *.
       cbn [tm_lvars tm_lvars_at value_lvars_at lvar_value_keys
         context_ty_lvars context_ty_lvars_at] in Hu |- *.
       apply elem_of_union in Hu as [Haτx|Hay_single].
@@ -133,10 +133,10 @@ Proof.
       unfold relevant_env, lty_env_restrict_lvars.
       rewrite storeA_restrict_lookup.
       destruct (decide
-        (LVFree a ∈ relevant_lvars (CTWand τx τ) (tret vf)))
+        (LVFree a ∈ context_tm_support (CTWand τx τ) (tret vf)))
         as [_|Hbad]; [reflexivity|].
       exfalso. apply Hbad.
-      unfold relevant_lvars in Hu |- *.
+      unfold relevant_lvars, context_tm_support in Hu |- *.
       cbn [tm_lvars tm_lvars_at value_lvars_at lvar_value_keys
         context_ty_lvars context_ty_lvars_at] in Hu |- *.
       apply elem_of_union in Hu as [Haτx|Hay_single].
@@ -199,11 +199,11 @@ Proof.
 	      * repeat rewrite lookup_insert_ne by congruence.
 	        unfold relevant_env, lty_env_restrict_lvars.
 	        rewrite storeA_restrict_lookup.
-	        destruct (decide
-	          (LVFree a ∈ relevant_lvars (CTArrow τx τ) (tret vf)))
+		        destruct (decide
+		          (LVFree a ∈ context_tm_support (CTArrow τx τ) (tret vf)))
 	          as [_|Hbad]; [reflexivity|].
 	        exfalso. apply Hbad.
-	        unfold relevant_lvars in Hu |- *.
+		        unfold relevant_lvars, context_tm_support in Hu |- *.
 	        cbn [tm_lvars tm_lvars_at value_lvars_at lvar_value_keys
 	          context_ty_lvars context_ty_lvars_at] in Hu |- *.
 	        apply elem_of_union in Hu as [Huτ|Hu_tm].
